```py
1.9. Starting from the definition of x ≡ y mod N (namely, that N divides x−y), 
justify the substitution rule
x ≡ x1 mod N, y ≡ y1 mod N    ⇒    x + y ≡ x1 + y1 mod N,
and also the corresponding rule for multiplication.
```
```py
solution:
1. Lets say x mod N  = a and y mod N = b
2. now x + y mod N = a + b
3. a can also be written as a = x1 mod N since x ≡ x1 (mod N)
4. similarly b can be written as b = y1 mod N since y ≡ y1 (mod N)
5. from 2, 3, and 4 we have (x + y) mod N = (x1 + y1) mod N
6. From 5. we conclude: x + y ≡ x1 + y1(mod N)

Now lets prove the rule for multiplication:
x*y ≡ x1*y1(mod N)

1. Lets say x mod N  = a and y mod N = b
2. Now x * y (mod N) = a * b
3. a can also be written as a = x1 mod N since x ≡ x1 (mod N)
4. similarly b can be written as b = y1 mod N since y ≡ y1 (mod N)
5. from 2, 3, & 4 we have (x * y) mod N = (x1 * y1) mod N
6. from 5 we conclude x*y ≡ x1*y1(mod N)

Q.E.D
```
